theories/lang/notation.v
@@ -69,7 +69,6 @@ Notation "fn: xl := e" := (fnrec: <> xl := e)%E
   (at level 102, xl at level 1, e at level 200) : expr_scope.
 Notation "fn: xl := e" := (fnrec: <> xl := e)%V
   (at level 102, xl at level 1, e at level 200) : val_scope.
-Notation "return:" := "return" : expr_scope.
 
 Notation "let: x := e1 'in' e2" :=
   ((Lam (@cons binder x%binder nil) e2%E) (@cons expr e1%E nil))
@@ -83,8 +82,10 @@ Notation "let: x := e1 'in' e2" :=
 Notation "e1 ;; e2" := (let: <> := e1 in e2)%V
   (at level 100, e2 at level 200, format "e1  ;;  e2") : val_scope.
 
-Notation "'jump' k : el" := (App (Seq Skip k%V) el%E)
-  (at level 100, k at level 1, el at level 10, format "'jump'  k :  el") : expr_scope.
+Notation "jump: k el" := (App (Seq Skip k%V) el%E)
+  (at level 100, k at level 1, el at level 10) : expr_scope.
+Notation "return: el" := (jump: (Var "return") el%E)%E
+  (at level 100, el at level 10) : expr_scope.
 Notation "letcont: k xl := e1 'in' e2" :=
   ((Lam (@cons binder k%binder nil) e2%E) [Rec k%binder xl%binder e1%E])
   (at level 102, k, xl at level 1, e1, e2 at level 150) : expr_scope.
